@prefix rdf: <http://www.w3.org/1999/02/22-rdf-syntax-ns#>.
@prefix rdfs: <http://www.w3.org/2000/01/rdf-schema#>.
@prefix xsd: <http://www.w3.org/2001/XMLSchema#>.
@prefix foaf: <http://xmlns.com/foaf/0.1/>.
@prefix dc: <http://purl.org/dc/elements/1.1/>.
@prefix dcterms: <http://purl.org/dc/terms/>.
@prefix skos: <http://www.w3.org/2004/02/skos/core#>.
@prefix cvstatus: <http://rs.tdwg.org/cv/status/>.

<http://rs.tdwg.org/cv/status/extant>
     skos:inScheme cvstatus:;
     rdfs:isDefinedBy cvstatus:;
     dcterms:isPartOf cvstatus:;
     rdf:value "extant";
     rdfs:label "extant"@en;
     skos:prefLabel "extant"@en;
     rdfs:comment "The species is known or thought very likely to occur presently in the area, which encompasses localities with current or recent (last 20-30 years) records where suitable habitat at appropriate altitudes remains."@en;
     skos:definition "The species is known or thought very likely to occur presently in the area, which encompasses localities with current or recent (last 20-30 years) records where suitable habitat at appropriate altitudes remains."@en;
     a skos:Concept.

<http://rs.tdwg.org/cv/status/extant.ttl>
     dc:format "text/turtle";
     dc:creator "Biodiversity Information Standards (TDWG)";
     rdfs:comment "Generated by Guid-O-Matic 2.0 https://github.com/baskaufs/guid-o-matic";
     dcterms:references <http://rs.tdwg.org/cv/status/extant>;
     dcterms:modified "2017-04-06T19:20:00-05:00"^^xsd:dateTime;
     a foaf:Document.

<http://rs.tdwg.org/cv/status/pextant>
     skos:inScheme cvstatus:;
     rdfs:isDefinedBy cvstatus:;
     dcterms:isPartOf cvstatus:;
     rdf:value "possibly extant";
     rdfs:label "possibly extant"@en;
     skos:prefLabel "possibly extant"@en;
     rdfs:comment "There is no record of the species in the area, but the species may possibly occur."@en;
     skos:definition "There is no record of the species in the area, but the species may possibly occur."@en;
     a skos:Concept.

<http://rs.tdwg.org/cv/status/pextant.ttl>
     dc:format "text/turtle";
     dc:creator "Biodiversity Information Standards (TDWG)";
     rdfs:comment "Generated by Guid-O-Matic 2.0 https://github.com/baskaufs/guid-o-matic";
     dcterms:references <http://rs.tdwg.org/cv/status/pextant>;
     dcterms:modified "2017-04-06T19:20:00-05:00"^^xsd:dateTime;
     a foaf:Document.

<http://rs.tdwg.org/cv/status/pextinct>
     skos:inScheme cvstatus:;
     rdfs:isDefinedBy cvstatus:;
     dcterms:isPartOf cvstatus:;
     rdf:value "possibly extinct";
     rdfs:label "possibly extinct"@en;
     skos:prefLabel "possibly extinct"@en;
     rdfs:comment "The species was formerly known or thought very likely to occur in the area (post 1500 AD), but it is most likely now extirpated from the area because habitat loss and/or other threats are thought likely to have extirpated the species, and there have been no confirmed recent records despite searches."@en;
     skos:definition "The species was formerly known or thought very likely to occur in the area (post 1500 AD), but it is most likely now extirpated from the area because habitat loss and/or other threats are thought likely to have extirpated the species, and there have been no confirmed recent records despite searches."@en;
     a skos:Concept.

<http://rs.tdwg.org/cv/status/pextinct.ttl>
     dc:format "text/turtle";
     dc:creator "Biodiversity Information Standards (TDWG)";
     rdfs:comment "Generated by Guid-O-Matic 2.0 https://github.com/baskaufs/guid-o-matic";
     dcterms:references <http://rs.tdwg.org/cv/status/pextinct>;
     dcterms:modified "2017-05-02T07:54:00-05:00"^^xsd:dateTime;
     a foaf:Document.

<http://rs.tdwg.org/cv/status/recentlyextinct>
     skos:inScheme cvstatus:;
     rdfs:isDefinedBy cvstatus:;
     dcterms:isPartOf cvstatus:;
     rdf:value "extinct post 1500";
     rdfs:label "extinct post 1500"@en;
     skos:prefLabel "extinct post 1500"@en;
     skos:broader cvstatus:extinct;
     rdfs:comment "The species was formerly known or thought very likely to occur in the area (post 1500 AD), but it has been confirmed that the species no longer occurs because exhaustive searches have failed to produce recent records, and the intensity and timing of threats could plausibly have extirpated the taxon."@en;
     skos:definition "The species was formerly known or thought very likely to occur in the area (post 1500 AD), but it has been confirmed that the species no longer occurs because exhaustive searches have failed to produce recent records, and the intensity and timing of threats could plausibly have extirpated the taxon."@en;
     a skos:Concept.

<http://rs.tdwg.org/cv/status/recentlyextinct.ttl>
     dc:format "text/turtle";
     dc:creator "Biodiversity Information Standards (TDWG)";
     rdfs:comment "Generated by Guid-O-Matic 2.0 https://github.com/baskaufs/guid-o-matic";
     dcterms:references <http://rs.tdwg.org/cv/status/recentlyextinct>;
     dcterms:modified "2017-04-06T19:20:00-05:00"^^xsd:dateTime;
     a foaf:Document.

<http://rs.tdwg.org/cv/status/extinct>
     skos:inScheme cvstatus:;
     rdfs:isDefinedBy cvstatus:;
     dcterms:isPartOf cvstatus:;
     rdf:value "extinct";
     rdfs:label "extinct"@en;
     skos:prefLabel "extinct"@en;
     rdfs:comment "The species was formerly known or thought very likely to occur in the area, but it has been confirmed that the species no longer occurs because exhaustive searches have failed to produce recent records, and the intensity and timing of threats could plausibly have extirpated the taxon."@en;
     skos:definition "The species was formerly known or thought very likely to occur in the area, but it has been confirmed that the species no longer occurs because exhaustive searches have failed to produce recent records, and the intensity and timing of threats could plausibly have extirpated the taxon."@en;
     a skos:Concept.

<http://rs.tdwg.org/cv/status/extinct.ttl>
     dc:format "text/turtle";
     dc:creator "Biodiversity Information Standards (TDWG)";
     rdfs:comment "Generated by Guid-O-Matic 2.0 https://github.com/baskaufs/guid-o-matic";
     dcterms:references <http://rs.tdwg.org/cv/status/extinct>;
     dcterms:modified "2017-04-06T19:20:00-05:00"^^xsd:dateTime;
     a foaf:Document.

<http://rs.tdwg.org/cv/status/uncertain>
     skos:inScheme cvstatus:;
     rdfs:isDefinedBy cvstatus:;
     dcterms:isPartOf cvstatus:;
     rdf:value "uncertain";
     rdfs:label "presence uncertain"@en;
     skos:prefLabel "presence uncertain"@en;
     rdfs:comment "A record exists of the species' presence in the area, but this record requires verification or is rendered questionable owing to uncertainty over the identity or authenticity of the record, or the accuracy of the location."@en;
     skos:definition "A record exists of the species' presence in the area, but this record requires verification or is rendered questionable owing to uncertainty over the identity or authenticity of the record, or the accuracy of the location."@en;
     a skos:Concept.

<http://rs.tdwg.org/cv/status/uncertain.ttl>
     dc:format "text/turtle";
     dc:creator "Biodiversity Information Standards (TDWG)";
     rdfs:comment "Generated by Guid-O-Matic 2.0 https://github.com/baskaufs/guid-o-matic";
     dcterms:references <http://rs.tdwg.org/cv/status/uncertain>;
     dcterms:modified "2017-04-06T19:20:00-05:00"^^xsd:dateTime;
     a foaf:Document.

<http://rs.tdwg.org/cv/status/absent>
     skos:inScheme cvstatus:;
     rdfs:isDefinedBy cvstatus:;
     dcterms:isPartOf cvstatus:;
     rdf:value "absent";
     rdfs:label "absent"@en;
     skos:prefLabel "absent"@en;
     rdfs:comment "Not present in a place at an occasion"@en;
     skos:definition "Not present in a place at an occasion"@en;
     a skos:Concept.

<http://rs.tdwg.org/cv/status/absent.ttl>
     dc:format "text/turtle";
     dc:creator "Biodiversity Information Standards (TDWG)";
     rdfs:comment "Generated by Guid-O-Matic 2.0 https://github.com/baskaufs/guid-o-matic";
     dcterms:references <http://rs.tdwg.org/cv/status/absent>;
     dcterms:modified "2017-04-06T19:20:00-05:00"^^xsd:dateTime;
     a foaf:Document.

<http://rs.tdwg.org/cv/status/null>
     skos:inScheme cvstatus:;
     rdfs:isDefinedBy cvstatus:;
     dcterms:isPartOf cvstatus:;
     rdf:value "null";
     rdfs:label "no value given"@en;
     skos:prefLabel "no value given"@en;
     rdfs:comment "Record did not include a value"@en;
     skos:definition "Record did not include a value"@en;
     a skos:Concept.

<http://rs.tdwg.org/cv/status/null.ttl>
     dc:format "text/turtle";
     dc:creator "Biodiversity Information Standards (TDWG)";
     rdfs:comment "Generated by Guid-O-Matic 2.0 https://github.com/baskaufs/guid-o-matic";
     dcterms:references <http://rs.tdwg.org/cv/status/null>;
     dcterms:modified "2017-04-21T05:17:00-05:00"^^xsd:dateTime;
     a foaf:Document.

<http://rs.tdwg.org/cv/status/inappropriate>
     skos:inScheme cvstatus:;
     rdfs:isDefinedBy cvstatus:;
     dcterms:isPartOf cvstatus:;
     rdf:value "inappropriate";
     rdfs:label "inappropriate"@en;
     skos:prefLabel "inappropriate"@en;
     rdfs:comment "Record included a value that was inappropriate for the occurrenceStatus property"@en;
     skos:definition "Record included a value that was inappropriate for the occurrenceStatus property"@en;
     a skos:Concept.

<http://rs.tdwg.org/cv/status/inappropriate.ttl>
     dc:format "text/turtle";
     dc:creator "Biodiversity Information Standards (TDWG)";
     rdfs:comment "Generated by Guid-O-Matic 2.0 https://github.com/baskaufs/guid-o-matic";
     dcterms:references <http://rs.tdwg.org/cv/status/inappropriate>;
     dcterms:modified "2017-04-21T05:17:00-05:00"^^xsd:dateTime;
     a foaf:Document.

